driver_model/driver_callScript.sml
@@ -14,7 +14,7 @@ call_tx_dr (dr:driver_state) (buffer:word8 list) =
 dr with dr_tx := dr.dr_tx with
 <| state := dr_tx_idle;
 data_buf := buffer;
-tx_left_length := LENGTH buffer |>`
+tx_cur_length := 0 |>`
 
 (* call_rx_dr: driver_state -> num -> driver_state *)
 val call_rx_dr_def = Define `
@@ -31,6 +31,6 @@ dr with dr_xfer := dr.dr_xfer with
 <| state := dr_xfer_idle;
 xfer_dataOUT_buf := buffer;
 xfer_dataIN_buf := [];
-xfer_left_length := LENGTH buffer|>`
+xfer_cur_length := 0 |>`
 
 val _ = export_theory();
