driver_model/driver_stateScript.sml
@@ -21,7 +21,7 @@ issue_wr_ch0conf_speed: bool |>`
 
 (* dr_tx_general_state: spi driver transimit function state flags *)
 val _ = Datatype ` dr_tx_general_state =
-| dr_tx_pre | dr_tx_idle | dr_tx_conf_issued | dr_tx_read_txs 
+| dr_tx_not_ready | dr_tx_pre | dr_tx_idle | dr_tx_conf_issued | dr_tx_read_txs 
 | dr_tx_check_txs | dr_tx_write_data | dr_tx_read_eot 
 | dr_tx_check_eot | dr_tx_issue_disable | dr_tx_reset_conf`
 
@@ -29,11 +29,11 @@ val _ = Datatype ` dr_tx_general_state =
 val _ = Datatype `dr_tx_state = <|
 state: dr_tx_general_state; 
 data_buf: word8 list;
-tx_left_length: num |>`
+tx_cur_length: num |>`
 
 (* dr_rx_general_state: spi driver receive function state flags *)
 val _ = Datatype `dr_rx_general_state = 
-| dr_rx_pre | dr_rx_idle | dr_rx_conf_issued | dr_rx_read_rxs 
+| dr_rx_not_ready | dr_rx_pre | dr_rx_idle | dr_rx_conf_issued | dr_rx_read_rxs 
 | dr_rx_check_rxs | dr_rx_read_rx0 | dr_rx_fetch_data 
 | dr_rx_issue_disable | dr_rx_reset_conf`
 
@@ -45,17 +45,17 @@ rx_left_length: num |>`
 
 (* dr_xfer_general_state: spi driver transfer(full-duplex) function state flags *)
 val _ = Datatype `dr_xfer_general_state =
-| dr_xfer_pre | dr_xfer_idle | dr_xfer_conf_issued | dr_xfer_read_txs
-| dr_xfer_check_txs | dr_xfer_write_dataO | dr_xfer_read_rxs
-| dr_xfer_check_rxs | dr_xfer_read_rx0 | dr_xfer_fetch_dataI
-| dr_xfer_issue_disable | dr_xfer_reset_conf`
+| dr_xfer_not_ready | dr_xfer_pre | dr_xfer_idle | dr_xfer_conf_issued 
+| dr_xfer_read_txs | dr_xfer_check_txs | dr_xfer_write_dataO 
+| dr_xfer_read_rxs | dr_xfer_check_rxs | dr_xfer_read_rx0 
+| dr_xfer_fetch_dataI | dr_xfer_issue_disable | dr_xfer_reset_conf`
 
 (* dr_xfer_state *)
 val _ = Datatype `dr_xfer_state = <|
 state: dr_xfer_general_state;
 xfer_dataIN_buf: word8 list;
 xfer_dataOUT_buf: word8 list;
-xfer_left_length : num |>`
+xfer_cur_length : num |>`
 
 (* driver_state: spi driver state, including init, tx, rx and xfer functions state *)
 val _ = Datatype `driver_state = <|
