ds_abs1/ds_abs1_rxScript.sml
@@ -19,12 +19,8 @@ SPI_ABS1_RX_ENABLE (ds_abs1:ds_abs1_state) =
 (* DRIVER_ABS1_RX_ENABLE: ds_abs1_state -> bool *)
 val DRIVER_ABS1_RX_ENABLE_def = Define `
 DRIVER_ABS1_RX_ENABLE (ds_abs1:ds_abs1_state) =
-((ds_abs1.ds_abs1_rx.state = abs1_rx_idle) \/
-(ds_abs1.ds_abs1_rx.state = abs1_rx_receive) \/
-(ds_abs1.ds_abs1_rx.state = abs1_rx_update) \/
-(ds_abs1.ds_abs1_rx.state = abs1_rx_ready) \/
+((ds_abs1.ds_abs1_rx.state = abs1_rx_ready) \/
 (ds_abs1.ds_abs1_rx.state = abs1_rx_fetch_data) \/
-(ds_abs1.ds_abs1_rx.state = abs1_rx_return) \/
 (ds_abs1.ds_abs1_rx.state = abs1_rx_done) \/
 (ds_abs1.ds_abs1_rx.state = abs1_rx_check_1) \/
 (ds_abs1.ds_abs1_rx.state = abs1_rx_check_2))`
@@ -107,40 +103,11 @@ case ds_abs1.ds_abs1_rx.state of
 
 
 (* tau_dr related functions *)
-(* driver_abs1_rx_idle_op: ds_abs1_state -> ds_abs1_state *)
-val driver_abs1_rx_idle_op_def = Define `
-driver_abs1_rx_idle_op (ds_abs1:ds_abs1_state) = 
-ds_abs1 with <| ds_abs1_rx := ds_abs1.ds_abs1_rx with
-rx_data_buffer := [];
-driver_abs1 := ds_abs1.driver_abs1 with
-<| dr_abs1_last_read_ad := (SOME SPI0_CH0STAT);
-   dr_abs1_last_read_v := (SOME 0w) |> |>`
-
-(* driver_abs1_rx_receive_op: ds_abs1_state -> ds_abs1_state *)
-val driver_abs1_rx_receive_op_def = Define `
-driver_abs1_rx_receive_op (ds_abs1:ds_abs1_state) =
-ds_abs1 with driver_abs1 := ds_abs1.driver_abs1 with
-<| dr_abs1_last_read_ad := (SOME SPI0_CH0STAT);
-   dr_abs1_last_read_v := (SOME 0w) |>`
-
-(* driver_abs1_rx_update_op: ds_abs1_state -> ds_abs1_state *)
-val driver_abs1_rx_update_op_def = Define `
-driver_abs1_rx_update_op (ds_abs1:ds_abs1_state) =
-ds_abs1 with driver_abs1 := ds_abs1.driver_abs1 with
-<| dr_abs1_last_read_ad := (SOME SPI0_CH0STAT);
-   dr_abs1_last_read_v := (SOME 0w) |>`
-
 (* driver_abs1_rx_ready_op: ds_abs1_state -> ds_abs1_state *)
 val driver_abs1_rx_ready_op_def = Define `
 driver_abs1_rx_ready_op (ds_abs1:ds_abs1_state) =
-if (ds_abs1.driver_abs1.dr_abs1_last_read_ad = (SOME SPI0_CH0STAT)) /\
-   (ds_abs1.driver_abs1.dr_abs1_last_read_v = (SOME 0w))
-then ds_abs1 with driver_abs1 := ds_abs1.driver_abs1 with
-     dr_abs1_last_read_v := (SOME 1w)
-else ds_abs1 with 
-<| ds_abs1_rx := ds_abs1.ds_abs1_rx with state := abs1_rx_fetch_data;
-   driver_abs1 := ds_abs1.driver_abs1 with
-<| dr_abs1_last_read_ad := (SOME SPI0_CH0STAT); dr_abs1_last_read_v := (SOME 1w) |> |>`
+ds_abs1 with ds_abs1_rx := ds_abs1.ds_abs1_rx with 
+state := abs1_rx_fetch_data`
 
 (* driver_abs1_rx_fetch_data_op: ds_abs1_state -> ds_abs1_state *)
 val driver_abs1_rx_fetch_data_op_def = Define `
@@ -150,13 +117,6 @@ ds_abs1 with ds_abs1_rx := ds_abs1.ds_abs1_rx with
    else abs1_rx_ready_for_reset;
    rx_data_buffer := ds_abs1.ds_abs1_rx.rx_data_buffer ++ [ds_abs1.spi_abs1.RX_SHIFT_REG]; 
    rx_left_length := ds_abs1.ds_abs1_rx.rx_left_length - 1 |>`
-
-(* driver_abs1_return_op: ds_abs1_state -> ds_abs1_state *)
-val driver_abs1_rx_return_op_def = Define `
-driver_abs1_rx_return_op (ds_abs1:ds_abs1_state) =
-ds_abs1 with driver_abs1 := ds_abs1.driver_abs1 with
-<| dr_abs1_last_read_ad := (SOME SPI0_CH0STAT);
-   dr_abs1_last_read_v := (SOME 0w) |>`
 
 (* driver_abs1_rx_done_op: ds_abs1_state -> ds_abs1_state *)
 val driver_abs1_rx_done_op_def = Define `
@@ -173,8 +133,7 @@ driver_abs1_rx_check_1_op (ds_abs1: ds_abs1_state) =
 ds_abs1 with ds_abs1_rx := ds_abs1.ds_abs1_rx with 
 <| state := if ds_abs1.ds_abs1_rx.rx_left_length > 1 then abs1_rx_update
    else abs1_rx_pre_reset;
-   rx_data_buffer := ds_abs1.ds_abs1_rx.rx_data_buffer ++ 
-                     [(w2w (THE ds_abs1.driver_abs1.dr_abs1_last_read_v):word8)];
+   rx_data_buffer := ds_abs1.ds_abs1_rx.rx_data_buffer ++ [ds_abs1.spi_abs1.RX_SHIFT_REG];
    rx_left_length := ds_abs1.ds_abs1_rx.rx_left_length - 1 |>`
 
 (* driver_abs1_rx_check_2_op: ds_abs1_state -> ds_abs1_state *)
@@ -183,8 +142,7 @@ driver_abs1_rx_check_2_op (ds_abs1: ds_abs1_state) =
 ds_abs1 with ds_abs1_rx := ds_abs1.ds_abs1_rx with
 <| state := if ds_abs1.ds_abs1_rx.rx_left_length > 1 then abs1_rx_ready
    else abs1_rx_reset;
-   rx_data_buffer := ds_abs1.ds_abs1_rx.rx_data_buffer ++
-                     [(w2w (THE ds_abs1.driver_abs1.dr_abs1_last_read_v):word8)];
+   rx_data_buffer := ds_abs1.ds_abs1_rx.rx_data_buffer ++ [ds_abs1.spi_abs1.RX_SHIFT_REG];
    rx_left_length := ds_abs1.ds_abs1_rx.rx_left_length - 1 |>`
 
 (* driver_abs1_rx_operations: ds_abs1_state -> ds_abs1_state *)
@@ -192,12 +150,12 @@ val driver_abs1_rx_operations_def = Define `
 driver_abs1_rx_operations (ds_abs1:ds_abs1_state) =
 case ds_abs1.ds_abs1_rx.state of
   | abs1_rx_pre => ds_abs1 with err := T
-  | abs1_rx_idle => driver_abs1_rx_idle_op ds_abs1
-  | abs1_rx_receive => driver_abs1_rx_receive_op ds_abs1
-  | abs1_rx_update => driver_abs1_rx_update_op ds_abs1
+  | abs1_rx_idle => ds_abs1 with err := T
+  | abs1_rx_receive => ds_abs1 with err := T
+  | abs1_rx_update => ds_abs1 with err := T
   | abs1_rx_ready => driver_abs1_rx_ready_op ds_abs1
   | abs1_rx_fetch_data => driver_abs1_rx_fetch_data_op ds_abs1
-  | abs1_rx_return => driver_abs1_rx_return_op ds_abs1
+  | abs1_rx_return => ds_abs1 with err := T
   | abs1_rx_done => driver_abs1_rx_done_op ds_abs1
   | abs1_rx_last => ds_abs1 with err := T
   | abs1_rx_check_1 => driver_abs1_rx_check_1_op ds_abs1
@@ -251,10 +209,7 @@ abs1_rx_done_op (ds_abs1:ds_abs1_state) (data:word8 option) =
 if (data <> NONE) then
 ds_abs1 with 
 <| ds_abs1_rx := ds_abs1.ds_abs1_rx with state := abs1_rx_check_1;
-   spi_abs1 := ds_abs1.spi_abs1 with RX_SHIFT_REG := THE data;
-   driver_abs1 := ds_abs1.driver_abs1 with
-   <| dr_abs1_last_read_ad := (SOME SPI0_RX0); 
-   dr_abs1_last_read_v := (SOME (w2w ds_abs1.spi_abs1.RX_SHIFT_REG)) |> |>
+   spi_abs1 := ds_abs1.spi_abs1 with RX_SHIFT_REG := THE data |>
 else ds_abs1`
 
 (* abs1_rx_last_op: ds_abs1_state -> word8 option -> ds_abs1_state *)
