ds_abs1/ds_abs1_stateScript.sml
@@ -11,14 +11,15 @@ val _ = new_theory "ds_abs1_state";
 
 (* ds_abs1_init_state: the state of ds_abs1 init automaton *)
 val _ = Datatype `ds_abs1_init_general_state =
-| abs1_init_pre | abs1_init_start | abs1_init_check | abs1_init_done`
+| abs1_init_pre | abs1_init_start | abs1_init_done`
 
 val _ = Datatype `ds_abs1_init_state = <|
 state : ds_abs1_init_general_state |>`
 
 (* ds_abs1_tx_state: the state of ds_abs1 tx automaton *)
 val _ = Datatype `ds_abs1_tx_general_state =
-| abs1_tx_pre | abs1_tx_idle | abs1_tx_prepare | abs1_tx_trans 
+| abs1_tx_not_ready | abs1_tx_pre | abs1_tx_idle | abs1_tx_prepare 
+| abs1_tx_trans | abs1_tx_data_1 | abs1_tx_data_2
 | abs1_tx_done_1 | abs1_tx_done_2 | abs1_tx_done_3
 | abs1_tx_check_1 | abs1_tx_check_2 | abs1_tx_check_3 
 | abs1_tx_next | abs1_tx_ready_for_reset | abs1_tx_reset`
@@ -26,11 +27,11 @@ val _ = Datatype `ds_abs1_tx_general_state =
 val _ = Datatype `ds_abs1_tx_state = <|
 state: ds_abs1_tx_general_state;
 tx_data_buffer: word8 list;
-tx_left_length: num |>`
+tx_cur_length: num |>`
 
 (* ds_abs1_rx_state: the state of ds_abs1 rx automaton *)
 val _ = Datatype `ds_abs1_rx_general_state =
-| abs1_rx_pre | abs1_rx_idle | abs1_rx_receive 
+| abs1_rx_not_ready | abs1_rx_pre | abs1_rx_idle | abs1_rx_receive 
 | abs1_rx_update | abs1_rx_ready | abs1_rx_fetch_data 
 | abs1_rx_return | abs1_rx_done | abs1_rx_last 
 | abs1_rx_check_1 | abs1_rx_check_2 | abs1_rx_pre_reset 
@@ -43,31 +44,32 @@ rx_left_length: num |>`
 
 (* ds_abs1_xfer_state: the state of ds_abs1 xfer automaton *)
 val _ = Datatype `ds_abs1_xfer_general_state =
-| abs1_xfer_pre | abs1_xfer_idle | abs1_xfer_prepare | abs1_xfer_trans
-| abs1_xfer_exchange | abs1_xfer_update | abs1_xfer_ready | abs1_xfer_fetch_data
-| abs1_xfer_next | abs1_xfer_next_write | abs1_xfer_done
-| abs1_xfer_ready_for_reset | abs1_xfer_reset`
+| abs1_xfer_not_ready | abs1_xfer_pre | abs1_xfer_idle | abs1_xfer_prepare 
+| abs1_xfer_trans | abs1_xfer_data | abs1_xfer_exchange | abs1_xfer_update 
+| abs1_xfer_ready | abs1_xfer_fetch_data | abs1_xfer_next | abs1_xfer_next_write 
+| abs1_xfer_done | abs1_xfer_ready_for_reset | abs1_xfer_reset`
 
 val _ = Datatype `ds_abs1_xfer_state = <|
 state: ds_abs1_xfer_general_state;
 xfer_dataIN_buffer: word8 list;
 xfer_dataOUT_buffer: word8 list;
-xfer_left_length: num |>`
+xfer_cur_length: num |>`
 
 val _ = Datatype `spi_abs1_state = <|
 TX_SHIFT_REG: word8;
 RX_SHIFT_REG: word8 |>`
 
-(* only used for internal states transition *)
+(* only used for internal states transition 
 val _ = Datatype `driver_abs1_state = <|
 dr_abs1_last_read_ad: word32 option;
 dr_abs1_last_read_v: word32 option |>`
+*)
 
 (* ds_abs1_state: the state of the spi controller and driver combined abstract level1 model *)
 val _ = Datatype `ds_abs1_state = <|
 err: bool;
 spi_abs1: spi_abs1_state;
-driver_abs1: driver_abs1_state; (* TO REMOVE*)
+(* driver_abs1: driver_abs1_state;  TO REMOVE*)
 ds_abs1_init: ds_abs1_init_state;
 ds_abs1_tx: ds_abs1_tx_state;
 ds_abs1_rx: ds_abs1_rx_state;
