ds_abs1/ds_abs1_xferScript.sml
@@ -9,7 +9,7 @@ val _ = new_theory "ds_abs1_xfer";
 val SPI_ABS1_XFER_ENABLE_def = Define `
 SPI_ABS1_XFER_ENABLE (ds_abs1:ds_abs1_state) =
 ((ds_abs1.ds_abs1_xfer.state = abs1_xfer_idle) \/
-(ds_abs1.ds_abs1_xfer.state = abs1_xfer_trans) \/
+(ds_abs1.ds_abs1_xfer.state = abs1_xfer_data) \/
 (ds_abs1.ds_abs1_xfer.state = abs1_xfer_update) \/
 (ds_abs1.ds_abs1_xfer.state = abs1_xfer_fetch_data) \/
 (ds_abs1.ds_abs1_xfer.state = abs1_xfer_next) \/
@@ -19,11 +19,7 @@ SPI_ABS1_XFER_ENABLE (ds_abs1:ds_abs1_state) =
 (* DRIVER_ABS1_XFER_ENABLE: ds_abs1_state -> bool *)
 val DRIVER_ABS1_XFER_ENABLE_def = Define `
 DRIVER_ABS1_XFER_ENABLE (ds_abs1:ds_abs1_state) =
-((ds_abs1.ds_abs1_xfer.state = abs1_xfer_idle) \/
-(ds_abs1.ds_abs1_xfer.state = abs1_xfer_prepare) \/
-(ds_abs1.ds_abs1_xfer.state = abs1_xfer_trans) \/
-(ds_abs1.ds_abs1_xfer.state = abs1_xfer_exchange) \/
-(ds_abs1.ds_abs1_xfer.state = abs1_xfer_update) \/
+((ds_abs1.ds_abs1_xfer.state = abs1_xfer_prepare) \/
 (ds_abs1.ds_abs1_xfer.state = abs1_xfer_ready) \/
 (ds_abs1.ds_abs1_xfer.state = abs1_xfer_fetch_data) \/
 (ds_abs1.ds_abs1_xfer.state = abs1_xfer_next) \/
@@ -32,7 +28,8 @@ DRIVER_ABS1_XFER_ENABLE (ds_abs1:ds_abs1_state) =
 (* COMB_ABS1_XFER_ENABLE: ds_abs1_state -> bool *)
 val COMB_ABS1_XFER_ENABLE_def = Define `
 COMB_ABS1_XFER_ENABLE (ds_abs1:ds_abs1_state) =
-((ds_abs1.ds_abs1_xfer.state = abs1_xfer_ready_for_reset) \/
+((ds_abs1.ds_abs1_xfer.state = abs1_xfer_trans) \/
+(ds_abs1.ds_abs1_xfer.state = abs1_xfer_ready_for_reset) \/
 (ds_abs1.ds_abs1_xfer.state = abs1_xfer_reset))`
 
 (* tau_spi related functions *)
@@ -42,17 +39,13 @@ spi_abs1_xfer_idle_op (ds_abs1:ds_abs1_state) =
 ds_abs1 with ds_abs1_xfer := ds_abs1.ds_abs1_xfer with
 state := abs1_xfer_prepare`
 
-(* spi_abs1_xfer_trans_op: ds_abs1_state -> ds_abs1_state *)
-(* TO-FIX false for bi-simulation *)
-val spi_abs1_xfer_trans_op_def = Define `
-spi_abs1_xfer_trans_op (ds_abs1:ds_abs1_state) =
-ds_abs1 with
-<| ds_abs1_xfer := ds_abs1.ds_abs1_xfer with
-<| state := abs1_xfer_exchange;
-   xfer_dataOUT_buffer := TL ds_abs1.ds_abs1_xfer.xfer_dataOUT_buffer;
-   xfer_left_length := ds_abs1.ds_abs1_xfer.xfer_left_length - 1 |>;
-   spi_abs1 := ds_abs1.spi_abs1 with
-   TX_SHIFT_REG := HD ds_abs1.ds_abs1_xfer.xfer_dataOUT_buffer |>`
+(* spi_abs1_xfer_data_op: ds_abs1_state -> ds_abs1_state *)
+val spi_abs1_xfer_data_op_def = Define `
+spi_abs1_xfer_data_op (ds_abs1:ds_abs1_state) =
+ds_abs1 with <| ds_abs1_xfer := ds_abs1.ds_abs1_xfer with 
+state := abs1_xfer_exchange;
+spi_abs1 := ds_abs1.spi_abs1 with
+TX_SHIFT_REG := (EL (ds_abs1.ds_abs1_xfer.xfer_cur_length - 1) (ds_abs1.ds_abs1_xfer.xfer_dataOUT_buffer))|>`
 
 (* spi_abs1_xfer_update_op: ds_abs1_state -> ds_abs1_state *)
 val spi_abs1_xfer_update_op_def = Define `
@@ -88,10 +81,12 @@ state := abs1_xfer_reset`
 val spi_abs1_xfer_operations_def = Define `
 spi_abs1_xfer_operations (ds_abs1:ds_abs1_state) =
 case ds_abs1.ds_abs1_xfer.state of 
+  | abs1_xfer_not_ready => ds_abs1 with err := T
   | abs1_xfer_pre => ds_abs1 with err := T
   | abs1_xfer_idle => spi_abs1_xfer_idle_op ds_abs1
   | abs1_xfer_prepare => ds_abs1 with err := T
-  | abs1_xfer_trans => spi_abs1_xfer_trans_op ds_abs1
+  | abs1_xfer_trans => ds_abs1 with err := T
+  | abs1_xfer_data => spi_abs1_xfer_data_op ds_abs1
   | abs1_xfer_exchange => ds_abs1 with err := T
   | abs1_xfer_update => spi_abs1_xfer_update_op ds_abs1
   | abs1_xfer_ready => ds_abs1 with err := T
@@ -104,69 +99,24 @@ case ds_abs1.ds_abs1_xfer.state of
 
 
 (* tau_driver related functions *)
-(* driver_abs1_xfer_idle_op: ds_abs1_state -> ds_abs1_state *)
-val driver_abs1_xfer_idle_op_def = Define `
-driver_abs1_xfer_idle_op (ds_abs1:ds_abs1_state) =
-ds_abs1 with <| ds_abs1_xfer := ds_abs1.ds_abs1_xfer with
-<| xfer_dataIN_buffer := [];
-   xfer_left_length := LENGTH ds_abs1.ds_abs1_xfer.xfer_dataOUT_buffer |>;
-   driver_abs1 := ds_abs1.driver_abs1 with
-<| dr_abs1_last_read_ad := (SOME SPI0_CH0STAT);
-   dr_abs1_last_read_v := (SOME 0w) |> |>`
-
 (* driver_abs1_xfer_prepare_op: ds_abs1_state -> ds_abs1_state *)
 val driver_abs1_xfer_prepare_op_def = Define `
 driver_abs1_xfer_prepare_op (ds_abs1:ds_abs1_state) =
-if (ds_abs1.driver_abs1.dr_abs1_last_read_ad = (SOME SPI0_CH0STAT)) /\
-   (ds_abs1.driver_abs1.dr_abs1_last_read_v = (SOME 0w))
-then ds_abs1 with driver_abs1 := ds_abs1.driver_abs1 with
-     dr_abs1_last_read_v := (SOME 2w)
-else ds_abs1 with 
-<| ds_abs1_xfer := ds_abs1.ds_abs1_xfer with state := abs1_xfer_trans;
-   driver_abs1 := ds_abs1.driver_abs1 with
-<| dr_abs1_last_read_ad := (SOME SPI0_CH0STAT);
-   dr_abs1_last_read_v := (SOME 2w) |> |>`
-
-(* driver_abs1_xfer_trans_op: ds_abs1_state -> ds_abs1_state *)
-val driver_abs1_xfer_trans_op_def = Define `
-driver_abs1_xfer_trans_op (ds_abs1:ds_abs1_state) =
-ds_abs1 with driver_abs1 := ds_abs1.driver_abs1 with
-<| dr_abs1_last_read_ad := (SOME SPI0_CH0STAT);
-   dr_abs1_last_read_v := (SOME 0w) |>`
-
-(* driver_abs1_xfer_exchange_op: ds_abs1_state -> ds_abs1_state *)
-val driver_abs1_xfer_exchange_op_def = Define `
-driver_abs1_xfer_exchange_op (ds_abs1:ds_abs1_state) =
-ds_abs1 with driver_abs1 := ds_abs1.driver_abs1 with
-<| dr_abs1_last_read_ad := (SOME SPI0_CH0STAT);
-   dr_abs1_last_read_v := (SOME 0w) |>`
-
-(* driver_abs1_xfer_update_op: ds_abs1_state -> ds_abs1_state *)
-val driver_abs1_xfer_update_op_def = Define `
-driver_abs1_xfer_update_op (ds_abs1:ds_abs1_state) =
-ds_abs1 with driver_abs1 := ds_abs1.driver_abs1 with
-<| dr_abs1_last_read_ad := (SOME SPI0_CH0STAT);
-   dr_abs1_last_read_v := (SOME 0w) |>`
+ds_abs1 with ds_abs1_xfer := ds_abs1.ds_abs1_xfer with 
+state := abs1_xfer_trans`
 
 (* driver_abs1_xfer_ready_op: ds_abs1_state -> ds_abs1_state *)
 val driver_abs1_xfer_ready_op_def = Define `
 driver_abs1_xfer_ready_op (ds_abs1:ds_abs1_state) =
-if (ds_abs1.driver_abs1.dr_abs1_last_read_ad = (SOME SPI0_CH0STAT)) /\
-   (ds_abs1.driver_abs1.dr_abs1_last_read_v = (SOME 0w))
-then ds_abs1 with driver_abs1 := ds_abs1.driver_abs1 with
-     dr_abs1_last_read_v := (SOME 1w)
-else ds_abs1 with
-<| ds_abs1_xfer := ds_abs1.ds_abs1_xfer with state := abs1_xfer_fetch_data;
-   driver_abs1 := ds_abs1.driver_abs1 with
-<| dr_abs1_last_read_ad := (SOME SPI0_CH0STAT);
-   dr_abs1_last_read_v := (SOME 1w) |> |> `
+ds_abs1 with ds_abs1_xfer := ds_abs1.ds_abs1_xfer with 
+state := abs1_xfer_fetch_data`
 
 (* driver_abs1_xfer_fetch_data_op: ds_abs1_state -> ds_abs1_state *)
 val driver_abs1_xfer_fetch_data_op_def = Define `
 driver_abs1_xfer_fetch_data_op (ds_abs1:ds_abs1_state) =
 ds_abs1 with ds_abs1_xfer := ds_abs1.ds_abs1_xfer with 
-<| state := if ds_abs1.ds_abs1_xfer.xfer_left_length > 0 then abs1_xfer_next
-   else abs1_xfer_ready_for_reset;
+<| state := if ds_abs1.ds_abs1_xfer.xfer_cur_length < (LENGTH (ds_abs1.ds_abs1_xfer.xfer_dataOUT_buffer)) 
+   then abs1_xfer_next else abs1_xfer_ready_for_reset;
    xfer_dataIN_buffer := ds_abs1.ds_abs1_xfer.xfer_dataIN_buffer ++ [ds_abs1.spi_abs1.RX_SHIFT_REG] |>`
 
 (* driver_abs1_xfer_next_op: ds_abs1_state -> ds_abs1_state *)
@@ -179,20 +129,22 @@ state := abs1_xfer_next_write`
 val driver_abs1_xfer_done_op_def = Define `
 driver_abs1_xfer_done_op (ds_abs1:ds_abs1_state) =
 ds_abs1 with ds_abs1_xfer := ds_abs1.ds_abs1_xfer with
-<| state := if ds_abs1.ds_abs1_xfer.xfer_left_length > 0 then abs1_xfer_prepare
-   else abs1_xfer_reset;
+<| state := if ds_abs1.ds_abs1_xfer.xfer_cur_length < (LENGTH (ds_abs1.ds_abs1_xfer.xfer_dataOUT_buffer)) 
+   then abs1_xfer_prepare else abs1_xfer_reset;
    xfer_dataIN_buffer := ds_abs1.ds_abs1_xfer.xfer_dataIN_buffer ++ [ds_abs1.spi_abs1.RX_SHIFT_REG] |>`
 
 (* driver_abs1_xfer_operations: ds_abs1_state -> ds_abs1_state *)
 val driver_abs1_xfer_operations_def = Define `
 driver_abs1_xfer_operations (ds_abs1:ds_abs1_state) =
 case ds_abs1.ds_abs1_xfer.state of
+  | abs1_xfer_not_ready => ds_abs1 with err := T
   | abs1_xfer_pre => ds_abs1 with err := T
-  | abs1_xfer_idle => driver_abs1_xfer_idle_op ds_abs1
+  | abs1_xfer_idle => ds_abs1 with err := T
   | abs1_xfer_prepare => driver_abs1_xfer_prepare_op ds_abs1
-  | abs1_xfer_trans => driver_abs1_xfer_trans_op ds_abs1
-  | abs1_xfer_exchange => driver_abs1_xfer_exchange_op ds_abs1
-  | abs1_xfer_update => driver_abs1_xfer_update_op ds_abs1
+  | abs1_xfer_trans => ds_abs1 with err := T
+  | abs1_xfer_data => ds_abs1 with err := T
+  | abs1_xfer_exchange => ds_abs1 with err := T
+  | abs1_xfer_update => ds_abs1 with err := T
   | abs1_xfer_ready => driver_abs1_xfer_ready_op ds_abs1
   | abs1_xfer_fetch_data => driver_abs1_xfer_fetch_data_op ds_abs1
   | abs1_xfer_next => driver_abs1_xfer_next_op ds_abs1
@@ -203,6 +155,13 @@ case ds_abs1.ds_abs1_xfer.state of
 
 
 (* tau_comb related functions *)
+(* comb_abs1_xfer_trans_op: ds_abs1_state -> ds_abs1_state *)
+val comb_abs1_xfer_trans_op_def = Define `
+comb_abs1_xfer_trans_op (ds_abs1:ds_abs1_state) =
+ds_abs1 with ds_abs1_xfer := ds_abs1.ds_abs1_xfer with
+<| state := abs1_xfer_data;
+   xfer_cur_length := ds_abs1.ds_abs1_xfer.xfer_cur_length + 1 |>`
+
 (* comb_abs1_xfer_ready_for_reset_op: ds_abs1_state -> ds_abs1_state *)
 val comb_abs1_xfer_ready_for_reset_op_def = Define `
 comb_abs1_xfer_ready_for_reset_op (ds_abs1:ds_abs1_state) =
@@ -218,7 +177,9 @@ state := abs1_xfer_pre`
 (* comb_abs1_xfer_operations: ds_abs1_state -> ds_abs1_state *)
 val comb_abs1_xfer_operations_def = Define `
 comb_abs1_xfer_operations (ds_abs1:ds_abs1_state) =
-if ds_abs1.ds_abs1_xfer.state = abs1_xfer_ready_for_reset
+if ds_abs1.ds_abs1_xfer.state = abs1_xfer_trans 
+then (comb_abs1_xfer_trans_op ds_abs1)
+else if ds_abs1.ds_abs1_xfer.state = abs1_xfer_ready_for_reset
 then (comb_abs1_xfer_ready_for_reset_op ds_abs1)
 else if ds_abs1.ds_abs1_xfer.state = abs1_xfer_reset
 then (comb_abs1_xfer_reset_op ds_abs1)
@@ -254,6 +215,6 @@ ds_abs1 with ds_abs1_xfer := ds_abs1.ds_abs1_xfer with
 <| state := abs1_xfer_idle;
    xfer_dataOUT_buffer := buffer;
    xfer_dataIN_buffer := [];
-   xfer_left_length := LENGTH buffer |>`
+   xfer_cur_length := 0 |>`
 
 val _ = export_theory();
