thm/abs1_comb_bisimulationScript.sml
@@ -4,10 +4,11 @@ open driver_stateTheory driver_relationTheory;
 open ds_abs1_stateTheory;
 open ref_relTheory;
 open ds_abs1_relTheory;
-open abs1_comb_hold_ref_rel_call_lblTheory;
-open abs1_comb_hold_ref_rel_trans_lblTheory;
+open ref_rel_holds_call_lblTheory;
+open ref_rel_holds_trans_lblTheory;
+open abs1_comb_hold_ref_rel_spi_trTheory;
 
-val _ = new_theory "abs1_comb_hold_ref_rel";
+val _ = new_theory "abs1_comb_bisimulation";
 
 (* bi-simulation: ds_abs1' exists when lbl is not tau *)
 val abs1_comb_hold_ref_rel_not_tau_lbl = store_thm("abs1_comb_hold_ref_rel_not_tau_lbl",
@@ -27,12 +28,6 @@ val abs1_comb_hold_ref_rel_driver_tr = store_thm("abs1_comb_hold_ref_rel_driver_
 ``!(spi:spi_state) (dr:driver_state) (ds_abs1:ds_abs1_state).
 (ref_rel ds_abs1 dr spi) /\ (driver_tr dr tau dr') ==>
 ?ds_abs1'. (ds_abs1_tr ds_abs1 tau ds_abs1') /\ (ref_rel ds_abs1' dr' spi)``,
-cheat);
-
-val abs1_comb_hold_ref_rel_spi_tr = store_thm("abs1_comb_hold_ref_rel_spi_tr",
-``!(spi:spi_state) (dr:driver_state) (ds_abs1:ds_abs1_state).
-(ref_rel ds_abs1 dr spi) /\ (spi_tr spi tau spi') ==>
-?ds_abs1'. (ds_abs1_tr ds_abs1 tau ds_abs1') /\ (ref_rel ds_abs1' dr spi')``,
 cheat);
 
 val abs1_comb_hold_ref_rel_WR_UP = store_thm("abs1_comb_hold_ref_rel_WR_UP",
@@ -117,9 +112,6 @@ val comb_abs1_hold_ref_rel = store_thm("comb_abs1_hold_ref_rel",
 (ref_rel ds_abs1 dr spi) /\ (ds_abs1_tr ds_abs1 lbl ds_abs1') ==>
 (?dr' spi'. (local_tr (dr, spi) lbl (dr', spi')) /\ (ref_rel ds_abs1' dr' spi'))``,
 cheat);
-<<<<<<< HEAD
 
-=======
->>>>>>> 0e90da248938a4568bb193f8b0aa2975919feb94
 
 val _ = export_theory();
