thm/abs1_comb_hold_ref_rel_spi_trScript.sml
@@ -1,4 +1,5 @@
 open HolKernel bossLib boolLib Parse;
+open wordsLib wordsTheory;
 open SPI_stateTheory SPI_relationTheory SPI_initTheory SPI_txTheory SPI_rxTheory
 SPI_xferTheory SPI_schedulerTheory;
 open driver_stateTheory driver_relationTheory;
@@ -9,48 +10,32 @@ open ref_relTheory;
 
 val _ = new_theory "abs1_comb_hold_ref_rel_spi_tr";
 
-(* a lemma: INIT_ENABLE => SPI_ABS1_INIT_ENABLE based on ref_rel *)
-val COMB_IMP_ABS1_INIT_ENABLE = store_thm("COMB_IMP_ABS1_INIT_ENABLE",
-``!(spi:spi_state) (dr:driver_state) (ds_abs1:ds_abs1_state).
-(ref_rel ds_abs1 dr spi) /\ (INIT_ENABLE spi) ==>
-(SPI_ABS1_INIT_ENABLE ds_abs1)``,
-rw [INIT_ENABLE_def, SPI_ABS1_INIT_ENABLE_def] >>
-`IS_INIT_REL ds_abs1 dr spi` by METIS_TAC [ref_rel_def] >> 
-FULL_SIMP_TAC std_ss [IS_INIT_REL_def] >>
-rw [] >|
-[Cases_on `dr.dr_init.state` >>
-rw [] >|
-[`spi.init.state <> init_start` by rw [] >>
-Cases_on `ds_abs1.ds_abs1_init.state` >>
-rw [],
-`spi.init.state <> init_start` by rw [] >>
-Cases_on `ds_abs1.ds_abs1_init.state` >>
-rw [],
-`spi.init.state <> init_setregs` by rw [] >>
-Cases_on `ds_abs1.ds_abs1_init.state` >>
-rw [],
-Cases_on `ds_abs1.ds_abs1_init.state` >>
-rw []],
-Cases_on `spi.init.state` >>
-rw []]);
+(* a lemma for w2w
+val w2w_word8 = store_thm("w2w_word8",
+``!(a:word8). a = (w2w (w2w a:word32):word8)``,
+SIMP_TAC (std_ss++WORD_BIT_EQ_ss) []);
+*)
 
-(* ds_abs1' exists when spi performs init tau transition *)
+(* ref_rel holds for ds_abs1 dr spi' in case of init tau transition *)
 val ref_rel_spi_init_tau = store_thm("ref_rel_spi_init_tau",
 ``!(spi:spi_state) (dr:driver_state) (ds_abs1:ds_abs1_state).
 (ref_rel ds_abs1 dr spi) /\ (INIT_ENABLE spi) ==>
-?ds_abs1'. (ds_abs1_tr ds_abs1 tau ds_abs1') /\
-(ref_rel ds_abs1' dr (spi_init_operations spi))``,
-rw [ds_abs1_tr_cases, ds_abs1_spi_tr_cases] >>
-EXISTS_TAC ``spi_abs1_init_operations ds_abs1`` >>
-`SPI_ABS1_INIT_ENABLE ds_abs1` by METIS_TAC [COMB_IMP_ABS1_INIT_ENABLE] >>
-rw [] >>
-FULL_SIMP_TAC std_ss [INIT_ENABLE_def, SPI_ABS1_INIT_ENABLE_def] >>
-rw [spi_abs1_init_operations_def, spi_abs1_init_start_op_def,
-spi_init_operations_def, init_reset_op_def] >>
+(ref_rel ds_abs1 dr (spi_init_operations spi))``,
+rw [INIT_ENABLE_def, spi_init_operations_def, init_reset_op_def] >>
 FULL_SIMP_TAC std_ss [ref_rel_def] >>
+rw [] >|
+[FULL_SIMP_TAC std_ss [IS_INIT_REL_def] >>
 rw [] >>
-FULL_SIMP_TAC std_ss [IS_INIT_REL_def, IS_TX_REL_def, IS_RX_REL_def, IS_XFER_REL_def] >>
-rw []);
+Cases_on `ds_abs1.ds_abs1_init.state` >>
+rw [] >>
+rw [],
+FULL_SIMP_TAC std_ss [IS_TX_REL_def] >>
+rw [],
+FULL_SIMP_TAC std_ss [IS_RX_REL_def] >>
+rw [],
+FULL_SIMP_TAC std_ss [IS_XFER_REL_def] >>
+rw []]);
+
 
 (* a lemma: TX_ENABLE => SPI_ABS1_TX_ENABLE based on ref_rel *)
 val COMB_IMP_ABS1_TX_ENABLE = store_thm("COMB_IMP_ABS1_TX_ENABLE",
@@ -86,13 +71,22 @@ FULL_SIMP_TAC std_ss [ref_rel_def] >>
 rw [] >>
 FULL_SIMP_TAC std_ss [IS_INIT_REL_def, IS_TX_REL_def, IS_RX_REL_def, IS_XFER_REL_def] >>
 rw [],
-(* abs1_tx_trans_data *)
+(* abs1_tx_data_1 *)
 `spi.tx.state = tx_trans_data` by METIS_TAC [ref_rel_def, IS_TX_REL_def] >>
-rw [spi_abs1_tx_operations_def, spi_abs1_tx_trans_op_def,
+rw [spi_abs1_tx_operations_def, spi_abs1_tx_data_1_op_def,
 spi_tx_operations_def, tx_trans_data_op_def] >>
 FULL_SIMP_TAC std_ss [ref_rel_def] >>
 rw [] >>
-cheat,
+FULL_SIMP_TAC std_ss [IS_INIT_REL_def, IS_TX_REL_def, IS_RX_REL_def, IS_XFER_REL_def] >>
+rw [],
+(* abs1_tx_data_2 *)
+`spi.tx.state = tx_trans_data` by METIS_TAC [ref_rel_def, IS_TX_REL_def] >>
+rw [spi_abs1_tx_operations_def, spi_abs1_tx_data_2_op_def,
+spi_tx_operations_def, tx_trans_data_op_def] >>
+FULL_SIMP_TAC std_ss [ref_rel_def] >>
+rw [] >>
+FULL_SIMP_TAC std_ss [IS_INIT_REL_def, IS_TX_REL_def, IS_RX_REL_def, IS_XFER_REL_def] >>
+rw [],
 (* abs1_tx_check_1 *)
 `spi.tx.state = tx_trans_check` by METIS_TAC [ref_rel_def, IS_TX_REL_def] >>
 rw [spi_abs1_tx_operations_def, spi_abs1_tx_check_1_op_def,
@@ -244,15 +238,15 @@ FULL_SIMP_TAC std_ss [ref_rel_def] >>
 rw [] >>
 FULL_SIMP_TAC std_ss [IS_INIT_REL_def, IS_TX_REL_def, IS_RX_REL_def, IS_XFER_REL_def] >>
 rw [],
-(* abs1_xfer_trans *)
+(* abs1_xfer_data *)
 `spi.xfer.state = xfer_trans_data` by METIS_TAC [ref_rel_def, IS_XFER_REL_def] >>
-rw [spi_abs1_xfer_operations_def, spi_abs1_xfer_trans_op_def,
+rw [spi_abs1_xfer_operations_def, spi_abs1_xfer_data_op_def,
 spi_xfer_operations_def, xfer_trans_data_op_def] >>
 FULL_SIMP_TAC std_ss [ref_rel_def] >>
 rw [] >>
-FULL_SIMP_TAC std_ss [IS_INIT_REL_def, IS_TX_REL_def, IS_RX_REL_def, IS_XFER_REL_def] >>
+FULL_SIMP_TAC std_ss [ref_rel_def,IS_INIT_REL_def, IS_TX_REL_def, IS_RX_REL_def, IS_XFER_REL_def] >>
 rw [] >>
-cheat,
+METIS_TAC[],
 (* abs1_xfer_update *)
 `spi.xfer.state = xfer_update_RX0` by METIS_TAC [ref_rel_def, IS_XFER_REL_def] >>
 rw [spi_abs1_xfer_operations_def, spi_abs1_xfer_update_op_def,
@@ -298,7 +292,8 @@ rw []]);
 val abs1_comb_hold_ref_rel_spi_tr = store_thm("abs1_comb_hold_ref_rel_spi_tr",
 ``!(spi:spi_state) (dr:driver_state) (ds_abs1:ds_abs1_state).
 (ref_rel ds_abs1 dr spi) /\ (spi_tr spi tau spi') ==>
-?ds_abs1'. (ds_abs1_tr ds_abs1 tau ds_abs1') /\ (ref_rel ds_abs1' dr spi')``,
+(ref_rel ds_abs1 dr spi') \/
+(?ds_abs1'. (ds_abs1_tr ds_abs1 tau ds_abs1') /\ (ref_rel ds_abs1' dr spi'))``,
 rw [spi_tr_cases] >>
 rw [ref_rel_spi_init_tau, ref_rel_spi_tx_tau, 
 ref_rel_spi_rx_tau, ref_rel_spi_xfer_tau]);
